src/dafny/util/merkle.dfy
@@ -14,10 +14,6 @@
 
 // Contains relevant algorithms for manipulating merkle roots, proofs and trees.
 module Merkle {
-
-    // Defines the hash function used for Merklisation.
-    function Hash<T(==)>(lhs:T, rhs:T) : T
-
     // Compute the Merkle root for a given blob of data.  If the data is a
     // single element, then that is returned.  Otherwise, the blob is divided
     // evenly and the has of each sub root computed:
@@ -34,12 +30,43 @@ module Merkle {
     //        \        /
     //           root
     //
-    function Root<T(==)>(data: seq<T>) : T
+    function Root<T(==)>(data: seq<T>, hash: (T,T)->T) : T
+    // Cannot generate commitments for empty vectors.
     requires |data| > 0 {
         if |data| == 1 then data[0]
         else
             var pivot := |data| / 2;
-            Hash(Root(data[..pivot]),Root(data[pivot..]))
+            hash(Root(data[..pivot],hash),Root(data[pivot..],hash))
+    }
+
+    // Construct a proof of inclusion for the value at a given index in a blob
+    // of data.  This corresponds to a path through the Merkle Tree from the
+    // root to the given item.  For example, the proof that C is at index 2 in
+    // the array [A,B,C,D] looks like:
+    //
+    //        X
+    //       / \
+    //      /   \
+    //     Y     Z
+    //          / \
+    //         C   D
+    //
+    // Thus, the proof is [Y,C,D], where Y=Hash(A,B).
+    function Proof<T(==)>(data: seq<T>, i: nat, hash: (T,T)->T) : (p:seq<T>)
+    // Cannot generate proofs for empty vectors.
+    requires |data| > 0 && i < |data|
+    // A proof always contains at least one element!
+    ensures |p| > 0 {
+        var pivot := |data| / 2;
+        if |data| == 1 then data
+        else if i < pivot then
+            var lhs := Proof(data[..pivot],i,hash);
+            var rhs := Root(data[pivot..],hash);
+            lhs + [rhs]
+        else
+            var lhs := Root(data[..pivot],hash);
+            var rhs := Proof(data[pivot..],i-pivot,hash);
+            [lhs] + rhs
     }
 
     // Verify a proof of inclusion by calculating its corresponding root, such
@@ -57,15 +84,17 @@ module Merkle {
     // The original blob was [A,B,C,D] and X, Y and Z are internal hashes with X
     // being the Merkle root.  Then, a proof that C was in the original blob
     // data is [Y,C,D].
-    function Verify<T(==)>(proof: seq<T>) : T
+    function Verify<T(==)>(proof: seq<T>, hash: (T,T)->T) : T
     // A proof must contain at least one element!
     requires |proof| > 0
-    decreases |proof| {
+    // Every step decreases the size of the proof by one.
+    decreases |proof|
+    {
         if |proof| == 1 then proof[0]
         else
             var m := |proof| - 2;
             var n := |proof| - 1;
-            var acc := Hash(proof[m],proof[n]);
-            Verify(proof[..m]+[acc])
+            var acc := hash(proof[m],proof[n]);
+            Verify(proof[..m]+[acc], hash)
     }
 }
