src/test/merkle_tests.dfy
@@ -14,21 +14,39 @@
 include "utils.dfy"
 include "../dafny/util/merkle.dfy"
 
-// A very simple Merkle tree implementation using bytes as words.
-module ByteMerkle refines Merkle {
+// A very simple Merkle Tree implementation over byte blobs which uses exclusive
+// or as the hash.
+module ByteMerkle {
     import opened Utils
-    // Instantiate our Merkle system
-    type Word = n:nat | n < 256
+    import Merkle
+
+    // In our scheme, messages and hashes are bytes.
+    type byte = n:nat | n < 256
 
     // A very simple (and definitely not cryptographically strong) hash
     // function.
-    opaque function Hash(lhs: Word, rhs: Word) : Word {
+    function Hash(lhs: byte, rhs: byte) : byte {
         var l8 := lhs as bv8;
         var r8 := rhs as bv8;
-        (l8 ^ r8) as Word
+        (l8 ^ r8) as byte
     }
 
-    method {:test} test_roots() {
+    function Root(bytes: seq<byte>) : byte
+    requires |bytes| > 0 {
+        Merkle.Root(bytes,Hash)
+    }
+
+    function Proof(bytes: seq<byte>, i:nat) : seq<byte>
+    requires |bytes| > 0 && i < |bytes| {
+        Merkle.Proof(bytes,i,Hash)
+    }
+
+    function Verify(proof: seq<byte>) : byte
+    requires |proof| > 0 {
+        Merkle.Verify(proof,Hash)
+    }
+
+    method {:test} test_root() {
         AssertAndExpect(Root([0]) == 0);
         AssertAndExpect(Root([0,0]) == 0);
         AssertAndExpect(Root([1,0]) == 1);
@@ -36,17 +54,37 @@ module ByteMerkle refines Merkle {
         AssertAndExpect(Root([7,2]) == 5);
         AssertAndExpect(Root([1,255]) == 254);
         AssertAndExpect(Root([2,1,0]) == 3);
-        assert Root([7,2,1,0]) == Root([Root([7,2]),Root([1,0])]);
+        assert Merkle.Root([7,2,1,0],Hash) == Hash(Hash(7,2),Hash(1,0));
         AssertAndExpect(Root([7,2,1,0]) == 4);
     }
 
-    method {:test} test_proofs() {
+    method {:test} test_verify() {
         AssertAndExpect(Verify([0]) == 0);
         AssertAndExpect(Verify([1,0]) == 1);
-        assert Verify([2,1,0]) == Hash(2,Hash(1,0));
+        assert Merkle.Verify([2,1,0],Hash) == Hash(2,Hash(1,0));
         AssertAndExpect(Verify([2,1,0]) == 3);
         // Proof that either 1 or 0 is in [7,2,1,0]
-        assert Verify([5,1,0]) == Hash(5,Hash(1,0));
+        assert Merkle.Verify([5,1,0],Hash) == Hash(5,Hash(1,0));
         AssertAndExpect(Verify([5,1,0]) == 4);
+    }
+
+    method {:test} test_proof() {
+        // n = 1
+        AssertAndExpect(Proof([0],0) == [0]);
+        // n = 2
+        AssertAndExpect(Proof([0,1],0) == [0,1]);
+        AssertAndExpect(Proof([0,1],1) == [0,1]);
+        // n = 3
+        assert Merkle.Proof([0,1,2],0,Hash) == Merkle.Proof([0],0,Hash) + [Merkle.Root([1,2],Hash)];
+        AssertAndExpect(Proof([0,1,2],0) == [0,3]);
+        AssertAndExpect(Proof([0,1,2],1) == [0,1,2]);
+        AssertAndExpect(Proof([0,1,2],2) == [0,1,2]);
+        // n = 4
+        assert Merkle.Proof([0,1,2,3],0,Hash) == Merkle.Proof([0,1],0,Hash) + [Merkle.Root([2,3],Hash)];
+        AssertAndExpect(Proof([0,1,2,3],0) == [0,1,1]);
+        assert Merkle.Proof([0,1,2,3],1,Hash) == Merkle.Proof([0,1],0,Hash) + [Merkle.Root([2,3],Hash)];
+        AssertAndExpect(Proof([0,1,2,3],1) == [0,1,1]);
+        AssertAndExpect(Proof([0,1,2,3],2) == [1,2,3]);
+        AssertAndExpect(Proof([0,1,2,3],3) == [1,2,3]);
     }
 }
