src/dafny/ccs/blob_merklization.dfy
@@ -1,0 +1,65 @@
+/*
+ * Copyright 2023 ConsenSys Software Inc.
+ *
+ * Licensed under the Apache License, Version 2.0 (the "License"); you may
+ * not use this file except in compliance with the License. You may obtain
+ * a copy of the License at http://www.apache.org/licenses/LICENSE-2.0
+ *
+ * Unless required by applicable law or agreed to in writing, software dis-
+ * tributed under the License is distributed on an "AS IS" BASIS, WITHOUT
+ * WARRANTIES OR CONDITIONS OF ANY KIND, either express or implied. See the
+ * License for the specific language governing permissions and limitations
+ * under the License.
+ */
+include "vector_commitment.dfy"
+include "../util/merkle.dfy"
+
+// An abstract vector commitment scheme which uses Merkle Tree's as the
+// underlying technique.  To make a concrete scheme, one must define the type
+// of messages and hashes.  However, everything else is provided (including
+// proofs of correctness).
+module BlobMerklization refines VectorCommitmentScheme {
+    import Merkle
+    // The type of a hash used in this scheme.  For example, it could be a u256
+    // or something else.
+    type Hash(0,==)
+    // The notion of an empty hash is useful for defining witnesses, as required
+    // by Dafny.  It does not have any other concrete purpose.
+    const EMPTY_HASH : Hash
+    // A commitment in this scheme is simply a hash (i.e. a Merkle Proof).
+    type Commitment = Hash
+    // An opening is a sequence of hashes which form a merkle proof.
+    type Opening = s:seq<Hash> | |s| > 0 witness [EMPTY_HASH]
+
+    // Construct a commitment by computing its Merkle root.
+    function Commit(vec: seq<Message>) : Commitment {
+        // Hash original vector
+        var hvec := seq(|vec|, (i:nat) requires i<|vec| => Hasher(vec[i]));
+        // Construct root
+        Merkle.Root(hvec, HashJoin)
+    }
+
+    // Construct an opening by computing a Merkle Proof
+    function Open(vec: seq<Message>, i: nat) : Opening {
+        // Hash original vector
+        var hvec := seq(|vec|, (i:nat) requires i<|vec| => Hasher(vec[i]));
+        // Construct proof
+        Merkle.Proof(hvec,i,HashJoin)
+    }
+
+    // Verify an opening using the Merkle Proof
+    predicate Verify(c: Commitment, o: Opening, i: nat, m: Message) {
+        i < |o| && o[i] == Hasher(m) && Merkle.Verify(o,HashJoin) == c
+    }
+
+    lemma {:verify false} Completeness(vec: seq<Message>, c: Commitment, o: Opening, i: nat, m: Message)
+    {
+        // FIXME: how to prove this?
+    }
+
+    // Defines the hash function used to convert messages into hashes.
+    function Hasher(lhs:Message) : Hash
+
+    // Defines the hash function used for joining hashes together.
+    function HashJoin(lhs:Hash, rhs:Hash) : Hash
+}
